format-version: 1.2
saved-by: cooperl
default-namespace: CO_325_banana
ontology: co_325

[Term]
id: CO_325:0000000
name: banana time from planting to shooting trait
def: "The time elapsed from planting to shooting (when the inflorescence emerges from the pseudostem and is still in an erect position)." [CO:curators]
synonym: "plant2shoot" EXACT []
is_a: TO:0000933 ! plant phenological trait

[Term]
id: CO_325:0000003
name: banana time from shooting to harvest trait
def: "The time elapsed from shooting (when the inflorescence emerges from the pseudostem and is still in an erect position) to the harvest of the bunch." [CO:curators]
synonym: "shoot2harvest" EXACT []
synonym: "time of fruit-filling, fruit-filling period, bunch maturity period, length of reproductive stage, bunch maturation period" EXACT []
is_a: TO:0000933 ! plant phenological trait

[Term]
id: CO_325:0000004
name: banana flowering trait
def: "whole-plant flowering related trait." [CO:curators]
is_a: TO:0002616 ! flowering time trait

[Term]
id: CO_325:0000006
name: banana plant crop cycle trait
def: "The time elapsed from planting to the harvest of the bunch." [CO:curators]
synonym: "Crop cycle, Mother plant crop cycle, Time from planting to harvest" EXACT []
synonym: "plant2harvest" EXACT []
is_a: TO:0000933 ! plant phenological trait

[Term]
id: CO_325:0000009
name: banana plant height trait
def: "The height of the pseudostem of the plant, from the collar to the intersection of the petioles of the two youngest leaves." [CO:curators]
synonym: "plantheightpetioles" EXACT []
synonym: "Pseudostem height" EXACT []
is_a: TO:0000207 ! plant height

[Term]
id: CO_325:0000012
name: banana plant circumference from the collar trait
def: "The circumference of the pseudostem of the plant." [CO:curators]
synonym: "Pseudostem girth, Plant circumference, Pseudostem circumference, Plant girth" EXACT []
is_a: TO:0000811 ! pseudostem diameter

[Term]
id: CO_325:0000021
name: banana monthly leaf emission rate trait
def: "A rate that expresses the number of leaves that have emerged from the pseudostem in a month." [CO:curators]
synonym: "LER" EXACT []
is_a: TO:0000735 ! plastochron

[Term]
id: CO_325:0000024
name: banana number of suckers trait
def: "The number of all types of suckers in the mat." [CO:curators]
synonym: "numsuckers" EXACT []
is_a: TO:0000077 ! shoot system morphology trait

[Term]
id: CO_325:0000027
name: banana tallest sucker height trait
def: "The height of the pseudostem of the tallest sucker within the same mat as the plant (the sucker that will become the next plant with a bunch, once the bunch from the current plant is harvested)." [CO:curators]
synonym: "Height of tallest sucker, Following sucker height, Height of following sucker" EXACT []
synonym: "suckerheight" EXACT []
is_a: TO:0000988 ! shoot-borne shoot system morphology trait

[Term]
id: CO_325:0000033
name: banana bunch weight trait
def: "The weight of the bunch, including the rachis." [CO:curators]
synonym: "bunchweight" EXACT []
is_a: TO:0000583 ! infructescence weight

[Term]
id: CO_325:0000036
name: banana number of hands in bunch trait
def: "The number of hands in the bunch." [CO:curators]
synonym: "numhands" EXACT []
is_a: TO:0000894 ! fruit number trait

[Term]
id: CO_325:0000039
name: banana number of fingers in bunch trait
def: "The number of fingers in the bunch." [CO:curators]
synonym: "numfingersbunch" EXACT []
is_a: TO:0000894 ! fruit number trait

[Term]
id: CO_325:0000042
name: banana number of fingers in hand: count trait
def: "The number of fingers in a third hand." [CO:curators]
synonym: "numfingershand" EXACT []
is_a: TO:0000894 ! fruit number trait

[Term]
id: CO_325:0000045
name: banana hand weight trait
def: "The weight of a hand." [CO:curators]
synonym: "handweight" EXACT []
is_a: TO:0000583 ! infructescence weight

[Term]
id: CO_325:0000048
name: banana finger weight trait
def: "The weight of a finger." [CO:curators]
synonym: "fingerweight" EXACT []
is_a: TO:0003031 ! pepo fruit weight

[Term]
id: CO_325:0000051
name: banana finger external length trait
def: "The length of a finger measured along the external (dorsal) arc, excluding the pedicel and the fruit tip." [CO:curators]
synonym: "Finger dorsal length" EXACT []
synonym: "fingerextlength" EXACT []
is_a: TO:0001098 ! pepo fruit morphology trait

[Term]
id: CO_325:0000054
name: banana finger circumference trait
def: "The circumference of a finger." [CO:curators]
synonym: "Finger girth" EXACT []
synonym: "fingercircumf" EXACT []
is_a: TO:0001098 ! pepo fruit morphology trait

[Term]
id: CO_325:0000057
name: banana black leaf streak disease incubation time trait
def: "The time elapsed between a tagged cigar leaf at Brun's stage B of unrolling and the development of black leaf streak disease symptoms at Foure's black leaf streak disease severity grade 1." [CO:curators]
synonym: "Black Sigatoka disease incubation time" EXACT []
synonym: "DIT" EXACT []
is_a: TO:0001145 ! Ascomycete fungal disease response

[Term]
id: CO_325:0000060
name: banana black leaf streak disease evolution time trait
def: "The time elapsed between the development of black leaf streak disease symptoms at Foure's black leaf streak disease severity grade 1, to 6." [CO:curators]
synonym: "Black Sigatoka disease evolution time" EXACT []
synonym: "DET" EXACT []
is_a: TO:0001145 ! Ascomycete fungal disease response

[Term]
id: CO_325:0000066
name: banana number of functional leaves trait
def: "The number of leaves on the plant that have 50% or more of the leaf surface area as green, healthy, photosynthetic tissue." [CO:curators]
synonym: "functleaves" EXACT []
synonym: "numFuncLeaves" EXACT []
is_a: TTO:0000241 ! leaf number

[Term]
id: CO_325:0000069
name: banana number of standing leaves trait
def: "The number of leaves attached to the plant that have an erect petiole (not bent or broken)." [CO:curators]
is_a: TTO:0000241 ! leaf number

[Term]
id: CO_325:0000072
name: banana extent of internal discolouration in corm of tallest sucker caused by fusarium wilt trait
def: "The extent of discolouration in the corm of the tallest sucker, caused by Fusarium wilt." [CO:curators]
is_a: TO:0001145 ! Ascomycete fungal disease response

[Term]
id: CO_325:0000075
name: banana distance of internal discolouration in pseudostem of plant caused by fusarium wilt trait
def: "The distance of discolouration in the pseudostem of the plant, caused by Fusarium wilt." [CO:curators]
is_a: TO:0001145 ! Ascomycete fungal disease response

[Term]
id: CO_325:0000078
name: banana percentage of plants with external disease symptoms caused by fusarium wilt trait
def: "The percentage of plants with any or multiple of the external disease symptoms - yellowing leaves, splitting of pseudostem base, changes in new leaves, petiole collapse, caused by Fusarium wilt." [CO:curators]
is_a: TO:0001145 ! Ascomycete fungal disease response

[Term]
id: CO_325:0000081
name: banana percentage of plants with internal disease symptoms caused by fusarium wilt trait
def: "The percentage of plants with any or multiple of the internal disease symptoms - discolouration in the corm, and/or discolouration in the pseudostem, caused by Fusarium wilt." [CO:curators]
is_a: TO:0001145 ! Ascomycete fungal disease response

[Term]
id: CO_325:0000084
name: banana time from start of crop cycle to first external disease symptoms caused by fusarium wilt trait
def: "The time elapsed from the start of the crop cycle to the appearance on the plant of any of the external disease symptoms - - yellowing leaves, splitting pseudostem base, changes in new leaves, petiole collapse, caused by Fusarium wilt." [CO:curators]
is_a: TO:0001145 ! Ascomycete fungal disease response

[Term]
id: CO_325:0000087
name: banana presence of yellowing leaves caused by fusarium wilt trait
def: "The presence/absence of yellowing leaves, caused by Fusarium wilt." [CO:curators]
synonym: "YL" EXACT []
is_a: TO:0001145 ! Ascomycete fungal disease response

[Term]
id: CO_325:0000090
name: banana presence of splitting pseudostem base caused by fusarium wilt trait
def: "The presence/absence of a splitting pseudostem base, caused by Fusarium wilt." [CO:curators]
synonym: "SP" EXACT []
is_a: TO:0001145 ! Ascomycete fungal disease response

[Term]
id: CO_325:0000093
name: banana presence of changes in new leaves caused by fusarium wilt trait
def: "The presence/absence of changes in new leaves - irregular pale margins, narrowing of lamina, burning plus ripping of lamina, lamina becoming more erect, caused by Fusarium wilt." [CO:curators]
synonym: "CNL" EXACT []
is_a: TO:0001145 ! Ascomycete fungal disease response

[Term]
id: CO_325:0000096
name: banana presence of petiole collapse caused by fusarium wilt trait
def: "The presence/absence of petiole collapse, caused by Fusarium wilt." [CO:curators]
synonym: "PC" EXACT []
is_a: TO:0001145 ! Ascomycete fungal disease response

[Term]
id: CO_325:0000099
name: banana youngest leaf spotted trait
def: "The rank (order) of the first fully unfurled leaf with at least 10 discrete, mature, necrotic lesions or one large necrotic area with 10 leaf spot light-coloued dry centres, caused by black leaf streak disease." [CO:curators]
synonym: "YLS" EXACT []
is_a: TO:0001145 ! Ascomycete fungal disease response

[Term]
id: CO_325:0000102
name: banana index of non-spotted leaves trait
def: "An index to express the proportion of standing leaves without the typical late-stage symptoms of black leaf streak disease, i.e. a black spot with a necrotic centre. This index provides an estimation of available photosynthetic leaf area prior to fruit filling and is a measure of resistance. It also corrects for the difference in the number of leaves produced by different types of bananas." [CO:curators]
synonym: "INSL" EXACT []
is_a: TO:0001145 ! Ascomycete fungal disease response

[Term]
id: CO_325:0000105
name: banana black leaf streak disease severity index trait
def: "An index to express the degree of leaf area of all standing leaves on the plant affected by black leaf streak disease." [CO:curators]
synonym: "Black Sigatoka disease infection index" EXACT []
is_a: TO:0001145 ! Ascomycete fungal disease response

[Term]
id: CO_325:0000108
name: banana number of dead roots trait
def: "The number of dead roots in a standard-size excavation of 20 x 20 x 20 cm extending outwards from the corm of the plant." [CO:curators]
is_a: TO:0001042 ! root quality trait

[Term]
id: CO_325:0000111
name: banana number of functional roots trait
def: "The number of functional roots in a standard-size excavation of 20 x 20 x 20 cm extending outwards from the corm of the plant." [CO:curators]
is_a: TO:0001042 ! root quality trait

[Term]
id: CO_325:0000114
name: banana number of all roots trait
def: "The total number of all roots (both dead and functional) in a standard-size excavation of 20 x 20 x 20 cm extending outwards from the corm of the plant." [CO:curators]
is_a: TO:0000084 ! root number

[Term]
id: CO_325:0000117
name: banana percentage of functional roots trait
def: "The percentage of all roots in a standard-size excavation of 20 x 20 x 20 cm extending outwards from the corm of the plant that are functional." [CO:curators]
is_a: TO:0001042 ! root quality trait

[Term]
id: CO_325:0000120
name: banana percentage of dead roots trait
def: "The percentage of the root cortex of five functional roots approximately 10 cm long that is necrotic due to nematode damage." [CO:curators]
is_a: TO:0001042 ! root quality trait

[Term]
id: CO_325:0000123
name: banana root necrosis caused by nematodes trait
def: "The percentage of the root cortex of five functional roots approximately 10 cm long that is necrotic due to nematode damage." [CO:curators]
is_a: TO:0000384 ! nematode damage response trait

[Term]
id: CO_325:0000126
name: banana nematode root knot galling extent trait
def: "The extent of root knot nematodes, observed externally as galls on the roots." [CO:curators]
is_a: TO:0000384 ! nematode damage response trait

[Term]
id: CO_325:0000129
name: banana nematode egg-laying females extent trait
def: "The extent of egg-laying female root knot nematodes, observed internally as pit-like structures on the roots." [CO:curators]
is_a: TO:0000384 ! nematode damage response trait

[Term]
id: CO_325:0000211
name: banana date of shooting trait
def: "The date the inflorescence emerges from the pseudostem and is still in an erect position." [CO:curators]
is_a: TO:0001021 ! days to inflorescence exsertion

[Term]
id: CO_325:0000218
name: banana date of flowering trait
def: "The date the last bracts fall from the most distal hand (closest to the male bud) to display the female flowers." [CO:curators]
is_a: TO:0002616 ! flowering time trait

[Term]
id: CO_325:0000221
name: banana number of maiden suckers trait
def: "The number of maiden suckers (fully grown suckers with foliage leaves) in the mat." [CO:curators]
synonym: "nummaidensuckers" EXACT []
is_a: TO:0000077 ! shoot system morphology trait

[Term]
id: CO_325:0000225
name: banana number of sword suckers trait
def: "The number of sword suckers (suckers with narrow leaves and a large rhizome) in the mat." [CO:curators]
synonym: "numswordsuckers" EXACT []
is_a: TO:0000077 ! shoot system morphology trait

[Term]
id: CO_325:0000229
name: banana number of peeper suckers trait
def: "The number of peeper suckers (suckers < 15 cm tall) in the mat." [CO:curators]
synonym: "numpeepersuckers" EXACT []
is_a: TO:0000077 ! shoot system morphology trait

[Term]
id: CO_325:0000233
name: banana finger lateral diameter trait
def: "The lateral (side to side) diameter of a finger." [CO:curators]
synonym: "Finger grade, Fruit diameter, Fruit grade" EXACT []
synonym: "fingerlatdiam" EXACT []
is_a: TO:0000848 ! fruit diameter

[Term]
id: CO_325:0000236
name: banana finger peel thickness trait
def: "The thickness of the peel of a finger." [CO:curators]
synonym: "peelthickness" EXACT []
synonym: "Width of the peel, Width of the skin, Width of the exocarp, Finger peel thickness" EXACT []
is_a: TO:0000907 ! exocarp thickness

[Term]
id: CO_325:0000240
name: banana fruit pulp lateral diameter trait
def: "The lateral (side to side) diameter of the pulp of a fruit." [CO:curators]
synonym: "Finger pulp diameter" EXACT []
synonym: "pulpdiam" EXACT []
is_a: TO:0001098 ! pepo fruit morphology trait

[Term]
id: CO_325:0000243
name: banana main underlying colour of pseudostem trait
def: "Main colour of the pseudostem under the outermost sheath." [CO:curators]
synonym: "Predominant underlying colour of the pseudostem" EXACT []
is_a: TO:0000810 ! pseudostem color

[Term]
id: CO_325:0000248
name: banana colour line along edge of petiole margin trait
def: "Presence or absence of colour line along edge of petiole margin." [CO:curators]
synonym: "Edge of petiole margin" EXACT []
is_a: TO:0000765 ! petiole morphology trait

[Term]
id: CO_325:0000250
name: banana pulp weight trait
def: "Peel the fruit and weigh the pulp using a scale (g). Record the pulp weight (g) of the central external finger on the second top cluster." [CO:curators]
synonym: "pulpweight" EXACT []
is_a: TO:0003031 ! pepo fruit weight

[Term]
id: CO_325:0000252
name: banana pigmentation of outer surface of cigar leaf on sucker trait
def: "Colour of pigmentation on outer surface of cigar leaf on a developed sucker." [CO:curators]
synonym: "Colour of cigar leaf dorsal surface" EXACT []
is_a: TO:0000326 ! leaf color

[Term]
id: CO_325:0000256
name: banana petiole margins winged trait
def: "Behaviour of the petiole margins - winged or not winged. The petiole and pseudostem meet at shooting. Margin is the part of the petiole that can be bent outwards/inwards." [CO:curators]
synonym: "Petiole margins" EXACT []
is_a: TO:0000765 ! petiole morphology trait

[Term]
id: CO_325:0000260
name: banana petiole margins clasping trait
def: "Behaviour of the petiole margins - winged or not winged. the petiole and pseudostem meet at shooting. Margin is the part of the petiole that can be bent outwards/inwards." [CO:curators]
synonym: "Petiole margins" EXACT []
is_a: TO:0000765 ! petiole morphology trait

[Term]
id: CO_325:0000264
name: banana petiole margin colour trait
def: "Main colour of the petiole margin. Where the petiole and pseudostem meet at shooting. Margin is the part of the petiole that can be bent outwards/inwards." [CO:curators]
is_a: TO:0000765 ! petiole morphology trait

[Term]
id: CO_325:0000270
name: banana peel weight trait
def: "Weigh peel, using a scale (g). Record the peel weight (g) of the central external finger on the second top cluster." [CO:curators]
synonym: "peelweight" EXACT []
is_a: TO:0000906 ! exocarp morphology trait

[Term]
id: CO_325:0000292
name: banana time from flowering to harvest trait
def: "The time elapsed from flowering (when the last bracts fall from the most distal hand to display the female flowers) to the harvest of the bunch." [CO:curators]
synonym: "flower2harvest" EXACT []
is_a: TO:0000366 ! reproductive growth time

[Term]
id: CO_325:0000294
name: banana time from planting to death trait
def: "The time elapsed from planting to the death of the plant." [CO:curators]
synonym: "plant2death" EXACT []
synonym: "Time to death" EXACT []
is_a: TO:0000933 ! plant phenological trait

[Term]
id: CO_325:0000296
name: banana time from harvest to death trait
def: "The time elapsed from the harvest of the bunch of the plant from the preceding crop cycle to the death of the plant from the current crop cycle." [CO:curators]
synonym: "harvest2death" EXACT []
synonym: "Time to death of the ratoon plant" EXACT []
is_a: TO:0000933 ! plant phenological trait

[Term]
id: CO_325:0000298
name: banana ratoon crop cycle trait
def: "The time elapsed from the harvest of the bunch of the plant from the preceding crop cycle to the harvest of the bunch of the plant from the current crop cycle." [CO:curators]
synonym: "harvest2harvest" EXACT []
synonym: "Time from harvest to harvest" EXACT []
is_a: TO:0000933 ! plant phenological trait

[Term]
id: CO_325:0000307
name: banana plant height to neck of peduncle trait
def: "The height of the pseudostem of the plant from the collar to the curved neck of the peduncle." [CO:curators]
synonym: "plantheightneck" EXACT []
synonym: "Pseudostem height" EXACT []
is_a: TO:0000207 ! plant height

[Term]
id: CO_325:0000310
name: banana number of water suckers trait
def: "The number of water suckers (suckers with broad leaves, a small rhizome, and a weak connection to the plant) in the mat." [CO:curators]
synonym: "numwatersuckers" EXACT []
is_a: TO:0000077 ! shoot system morphology trait

[Term]
id: CO_325:0000312
name: banana bunch maturity stage at harvest trait
def: "The stage of maturity of the bunch at harvest." [CO:curators]
synonym: "bunchmaturity" EXACT []
synonym: "Stage of harvesting" EXACT []
is_a: TO:0001076 ! infructescence development trait

[Term]
id: CO_325:0000314
name: banana rachis weight trait
def: "The weight of the rachis." [CO:curators]
synonym: "rachisweight" EXACT []
is_a: TO:0000782 ! inflorescence axis morphology trait

[Term]
id: CO_325:0000316
name: banana total finger weight trait
def: "The weight of all the hands of the bunch, excluding the rachis." [CO:curators]
synonym: "Total fruit weight, Total hand weight" EXACT []
synonym: "totalfingerweight" EXACT []
is_a: TO:0003031 ! pepo fruit weight

[Term]
id: CO_325:0000318
name: banana hand rank trait
def: "The rank (order) of a hand in the bunch." [CO:curators]
synonym: "handid" EXACT []
is_a: TO:1000004 ! infructescence position

[Term]
id: CO_325:0000320
name: banana multiple number of fingers in hand trait
def: "The number of fingers in multiple hands." [CO:curators]
synonym: "multnumfingshand" EXACT []
is_a: TO:0000894 ! fruit number trait

[Term]
id: CO_325:0000322
name: banana number of hands measured trait
def: "The number of hands used to obtain a measurement." [CO:curators]
synonym: "numhandsmeas" EXACT []
is_a: TO:0000936 ! infructescence yield trait

[Term]
id: CO_325:0000324
name: banana average number of fingers in hand trait
def: "The average number of fingers in a hand." [CO:curators]
synonym: "avenumfingshand_rltv" EXACT []
is_a: TO:0000894 ! fruit number trait

[Term]
id: CO_325:0000327
name: banana multiple hand weight trait
def: "The weight of multiple hands." [CO:curators]
synonym: "multhandweight" EXACT []
is_a: TO:0000583 ! infructescence weight

[Term]
id: CO_325:0000329
name: banana average hand weight trait
def: "The average weight of the hands." [CO:curators]
synonym: "avehandweight" EXACT []
is_a: TO:0000583 ! infructescence weight

[Term]
id: CO_325:0000331
name: banana multiple finger weight trait
def: "The weight of multiple fingers." [CO:curators]
synonym: "multfingerweight" EXACT []
is_a: TO:0003031 ! pepo fruit weight

[Term]
id: CO_325:0000335
name: banana average finger weight trait
def: "The average weight of the fingers." [CO:curators]
synonym: "avefingerweight" EXACT []
is_a: TO:0003031 ! pepo fruit weight

[Term]
id: CO_325:0000337
name: banana average finger external length trait
def: "The average length of the fingers measured along the external (dorsal) arc, excluding the pedicel and the fruit tip." [CO:curators]
synonym: "avefingerextlength" EXACT []
synonym: "Average finger dorsal length" EXACT []
is_a: TO:0002626 ! fruit length

[Term]
id: CO_325:0000339
name: banana finger internal length trait
def: "The length of a finger measured along the internal (ventral) arc, excluding the pedicel and the fruit tip." [CO:curators]
synonym: "Finger ventral length" EXACT []
synonym: "fingerintlength" EXACT []
is_a: TO:0002626 ! fruit length

[Term]
id: CO_325:0000341
name: banana average finger internal length trait
def: "The average length of the fingers measured along the internal (ventral) arc, excluding the pedicel and the fruit tip." [CO:curators]
synonym: "avefingerintlength" EXACT []
synonym: "Average finger ventral length" EXACT []
is_a: TO:0002626 ! fruit length

[Term]
id: CO_325:0000344
name: banana average finger circumference trait
def: "The average circumference of the fingers." [CO:curators]
synonym: "avefingercircumf" EXACT []
synonym: "Average finger girth" EXACT []
is_a: TO:0001098 ! pepo fruit morphology trait

[Term]
id: CO_325:0000348
name: banana average finger lateral diameter trait
def: "The average lateral (side to side) diameter of a finger." [CO:curators]
synonym: "avefingerlatdiam" EXACT []
synonym: "Finger grade, Fruit diameter, Fruit grade" EXACT []
is_a: TO:0000848 ! fruit diameter

[Term]
id: CO_325:0000352
name: banana average fruit pulp lateral diameter trait
def: "The average lateral (side to side) diameter of the pulp of a fruit." [CO:curators]
synonym: "avepulpdiam" EXACT []
synonym: "Finger pulp diameter" EXACT []
is_a: TO:0000945 ! pericarp morphology trait

[Term]
id: CO_325:0000355
name: banana average finger peel thickness trait
def: "The average thickness of the peel of a finger." [CO:curators]
synonym: "avepeelthickness" EXACT []
synonym: "Width of the peel, Width of the skin, Width of the exocarp, Finger peel thickness" EXACT []
is_a: TO:0000907 ! exocarp thickness

[Term]
id: CO_325:0000381
name: banana annual crop cycle proportion trait
def: "The proportion of the crop cycle that takes place in one year." [CO:curators]
synonym: "anncropcycprop" EXACT []
is_a: TO:0000933 ! plant phenological trait

[Term]
id: CO_325:0000383
name: banana plant annual yield trait
def: "The bunch weight produced by the plant over the course of the crop cycle, averaged across one year." [CO:curators]
synonym: "plantannyield" EXACT []
is_a: TO:0000936 ! infructescence yield trait

[Term]
id: CO_325:0000385
name: banana average actual annual yield trait
def: "The average actual annual yield, taking into account the proportion of plants harvested, from the number of plants planted." [CO:curators]
synonym: "actualannyield" EXACT []
synonym: "Yield" EXACT []
is_a: TO:0000936 ! infructescence yield trait

[Term]
id: CO_325:0000387
name: banana average potential annual yield trait
def: "The average potential annual yield, assuming that all plants are harvested, from the number of plants planted." [CO:curators]
synonym: "potannyield" EXACT []
synonym: "Yield" EXACT []
is_a: TO:0000936 ! infructescence yield trait

[Term]
id: CO_325:0000389
name: banana overall fruit pendulance quality trait
def: "The overall estimation fruit pendulance on a bunch." [CO:curators]
synonym: "pendulantfruit" EXACT []
is_a: TO:0000920 ! infructescence morphology trait

[Term]
id: CO_325:0000391
name: banana overall bunch quality trait
def: "The overall estimation of the bunch quality on a mat." [CO:curators]
synonym: "goodbunch" EXACT []
is_a: TO:0002728 ! fruit quality

[Term]
id: CO_325:0000393
name: banana fruitfill trait
def: "The overall estimation of fruitfilling level on a bunch." [CO:curators]
synonym: "goodfruitfill" EXACT []
is_a: TO:0000929 ! fruit growth and development trait

[Term]
id: CO_325:0000395
name: banana overall suckering quality trait
def: "The overall estimation of sucker quality on a mat." [CO:curators]
synonym: "suckering" EXACT []
is_a: TO:0000988 ! shoot-borne shoot system morphology trait

[Term]
id: CO_325:0000397
name: banana dwarfism trait
def: "The presence or absence of dwarfism on a mat." [CO:curators]
synonym: "dwarfism" EXACT []
is_a: TO:0000398 ! whole plant morphology trait

[Term]
id: CO_325:0000425
name: banana pseudostem height trait
def: "Distance from the base of the pseudostem to the emerging point of the peduncle." [CO:curators]
synonym: "Plant height" EXACT []
is_a: TO:0000207 ! plant height

[Term]
id: CO_325:0000427
name: banana blotches relative area at petiole base trait
def: "Percentage coverage of petiole base by blotches." [CO:curators]
synonym: "Blotches at the petiole base" EXACT []
is_a: TO:0000765 ! petiole morphology trait

[Term]
id: CO_325:0000430
name: banana blotches colour at the petiole base trait
def: "Colour of the blotches on the upper leaf sheath of the petiole base." [CO:curators]
synonym: "Blotches colour" EXACT []
is_a: TO:0000765 ! petiole morphology trait

[Term]
id: CO_325:0000433
name: banana margin behaviour on petiole canal of third leaf trait
def: "Margin behaviour of the petiole canal of the third leaf before bunch." [CO:curators]
synonym: "Petiole canal of the third leaf, Petiole canal leaf III" EXACT []
is_a: TO:0000765 ! petiole morphology trait

[Term]
id: CO_325:0000438
name: banana bunch orientation trait
def: "Angle between the axis of the bunch and the vertical." [CO:curators]
is_a: TO:1000004 ! infructescence position

[Term]
id: CO_325:0000440
name: banana bunch shape trait
def: "Shape of the fully developed bunch on a plant." [CO:curators]
is_a: TO:0000920 ! infructescence morphology trait

[Term]
id: CO_325:0000442
name: banana male rachis type trait
def: "Behaviour of male rachis - truncated or present. Truncated means there is no bract scar below the last hand. Present means there is a degenerated or persistent male bud." [CO:curators]
is_a: TO:0000782 ! inflorescence axis morphology trait

[Term]
id: CO_325:0000444
name: banana male rachis position trait
def: "Angle of the rachis between last hand and male bud." [CO:curators]
synonym: "Rachis angle" EXACT []
is_a: TO:0000782 ! inflorescence axis morphology trait

[Term]
id: CO_325:0000446
name: banana male rachis appearance trait
def: "Appearance of flowers/bracts on the male rachis." [CO:curators]
synonym: "Rachis appearance" EXACT []
is_a: TO:0000782 ! inflorescence axis morphology trait

[Term]
id: CO_325:0000448
name: banana male bud shape trait
def: "Shape of the male bud defined as the ratio of male bud broadest width to total male bud length." [CO:curators]
is_a: TO:0000789 ! bud morphology trait

[Term]
id: CO_325:0000451
name: banana male bud length trait
def: "Length of male bud from end of rachis to apex of the bud." [CO:curators]
synonym: "Male bud size" EXACT []
is_a: TO:0000789 ! bud morphology trait

[Term]
id: CO_325:0000454
name: banana male bud shoulder trait
def: "Male bud shoulder description." [CO:curators]
synonym: "Male bud size" EXACT []
is_a: TO:0000789 ! bud morphology trait

[Term]
id: CO_325:0000456
name: banana bract apex shape trait
def: "Appearance of flowers/bracts on the male rachis." [CO:curators]
is_a: TO:0000816 ! inflorescence bract morphology trait

[Term]
id: CO_325:0000459
name: banana bract imbrication at apex of male bud trait
def: "Alignment of bracts at the apex of the male bud." [CO:curators]
synonym: "Bract imbrication" EXACT []
is_a: TO:0000816 ! inflorescence bract morphology trait

[Term]
id: CO_325:0000461
name: banana bract behaviour before falling trait
def: "Behaviour of the last lifted bract - revolute or not revolute." [CO:curators]
is_a: TO:0000816 ! inflorescence bract morphology trait

[Term]
id: CO_325:0000463
name: banana colour of bract external face trait
def: "Main colour of the first external unlifted bract external face." [CO:curators]
synonym: "Colour of the bract external face" EXACT []
is_a: TO:0000819 ! inflorescence bract color

[Term]
id: CO_325:0000466
name: banana colour of bract internal face trait
def: "Main colour of the first external unlifted bract internal face." [CO:curators]
synonym: "Colour of the bract internal face" EXACT []
is_a: TO:0000819 ! inflorescence bract color

[Term]
id: CO_325:0000469
name: banana compound tepal main colour trait
def: "Main colour of the backside of the compound tepal." [CO:curators]
synonym: "Tepal colour, Compound tepal basic colour" EXACT []
is_a: TO:0000574 ! tepal color

[Term]
id: CO_325:0000472
name: banana lobe colour of tip of compound tepal trait
def: "Main colour of the tip of the compound tepal (lobe)." [CO:curators]
synonym: "Lobe colour, Lobe colour of compound tepal" EXACT []
is_a: TO:0000574 ! tepal color

[Term]
id: CO_325:0000475
name: banana anther colour trait
def: "Main colour of the face of anther opposite to dehiscence." [CO:curators]
is_a: TO:0000187 ! anther color

[Term]
id: CO_325:0000478
name: banana number of hands on whole bunch trait
def: "number of hands on bunch **subsume." [CO:curators]
synonym: "number of hands" EXACT []
is_a: TO:0000894 ! fruit number trait

[Term]
id: CO_325:0000480
name: banana number of fruits on mid-hand of the bunch trait
def: "number of fruits on the mid-hand of the bunch **subsume." [CO:curators]
synonym: "number of fruits" EXACT []
is_a: TO:0000894 ! fruit number trait

[Term]
id: CO_325:0000482
name: banana fruit length trait
def: "Length of the internal arc of a finger ** subsume." [CO:curators]
synonym: "Fruit length" EXACT []
is_a: TO:0002626 ! fruit length

[Term]
id: CO_325:0000485
name: banana fruit shape of curve trait
def: "Shape of a fruit (finger) in the middle of the bunch **subsume." [CO:curators]
synonym: "Fruit shape (longitudinal curve)" EXACT []
is_a: TO:0002628 ! fruit shape

[Term]
id: CO_325:0000488
name: banana fruit apex point trait
def: "Description of fruit apex." [CO:curators]
synonym: "Fruit apex" EXACT []
is_a: TO:0001098 ! pepo fruit morphology trait

[Term]
id: CO_325:0000490
name: banana remains of flower relicts at fruit apex trait
def: "Percentage of flower relicts at fruit apex." [CO:curators]
is_a: TO:0001098 ! pepo fruit morphology trait

[Term]
id: CO_325:0000493
name: banana fruit pedicel length trait
def: "Length of the fruit pedicel from rachis to the beginning of the pulp." [CO:curators]
is_a:  TO:0000630 ! pedicel length

[Term]
id: CO_325:0000496
name: banana fusion of pedicels trait
def: "Degree of fusion of the pedicels before they join the rachis." [CO:curators]
is_a: TO:0000920 ! infructescence morphology trait

[Term]
id: CO_325:0000498 trait
name: banana fruit mashed pulp colour
def: "The color of the mashed pulp of a mature fruit." [CO:curators]
is_a: TO:0002619 ! mesocarp color

[Term]
id: CO_325:0000500 trait
name: banana fruit unmashed pulp colour
def: "The color of the unmashed pulp of a mature fruit." [CO:curators]
is_a: TO:0002619 ! mesocarp color

[Term]
id: CO_325:0000502
name: banana fruit mashed pulp taste trait
def: "The taste of the mashed pulp of a mature fruit." [CO:curators]
is_a: TO:0002694 ! fruit flavor trait

[Term]
id: CO_325:0000504
name: banana fruit unmashed pulp taste trait
def: "The taste of the unmashed pulp of a mature fruit." [CO:curators]
is_a: TO:0002694 ! fruit flavor trait

[Term]
id: CO_325:0000506
name: banana fruit mashed pulp texture trait
def: "The texture of the mashed pulp of a mature fruit." [CO:curators]
is_a: TO:0000948 ! mesocarp morphology trait

[Term]
id: CO_325:0000508
name: banana fruit unmashed pulp texture trait
def: "The texture of the unmashed pulp of a mature fruit." [CO:curators]
is_a: TO:0000948 ! mesocarp morphology trait

[Term]
id: CO_325:0000510
name: banana fruit mashed pulp smoothness-mouth feel trait
def: "The smoothness-mouth feel of the mashed pulp of a mature fruit." [CO:curators]
is_a: TO:0001098 ! pepo fruit morphology trait

[Term]
id: CO_325:0000512
name: banana fruit unmashed pulp smoothness-mouth feel trait
def: "The smoothness-mouth feel of the unmashed pulp of a mature fruit." [CO:curators]
is_a: TO:0001098 ! pepo fruit morphology trait

[Term]
id: CO_325:0000514
name: banana fruit mashed pulp aroma/smell trait
def: "The pulp aroma of the mashed pulp of a mature fruit." [CO:curators]
is_a: TO:0002694 ! fruit flavor trait

[Term]
id: CO_325:0000516
name: banana damage to periphery of peeled corm caused by weevils trait
def: "The amount of damage to the periphery of the peeled corm, assessed by tunnels caused by weevils." [CO:curators]
synonym: "peripheral damage" EXACT []
is_a: TO:0000261 ! insect damage response trait

[Term]
id: CO_325:0000518
name: banana nematode reproduction factor (microplot screening) trait
def: "Nematode multiplication from single root inoculation of 50 nematodes per 8 cm length after 12 weeks." [CO:curators]
is_a: TO:0000384 ! nematode damage response trait

[Term]
id: CO_325:0000520
name: banana nematode population density per soil sample trait
def: "number of nematodes in soil." [CO:curators]
is_a: TO:0000384 ! nematode damage response trait

[Term]
id: CO_325:0000524
name: banana number of rotylenchulus spp.per soil sample trait
def: "Number of Rotylenchulus spp.in soil." [CO:curators]
is_a: TO:0000384 ! nematode damage response trait

[Term]
id: CO_325:0000526
name: banana number of meloidogyne spp. per soil sample trait
def: "Number of Meloidogyne spp. in soil." [CO:curators]
is_a: TO:0000384 ! nematode damage response trait

[Term]
id: CO_325:0000528
name: banana number of hoplolaimus spp. per soil sample trait
def: "Number of Hoplolaimus spp. in soil." [CO:curators]
is_a: TO:0000384 ! nematode damage response trait

[Term]
id: CO_325:0000530
name: banana number of pratylenchus coffeae per soil sample trait
def: "Number of Pratylenchus coffeae in soil." [CO:curators]
is_a: TO:0000384 ! nematode damage response trait

[Term]
id: CO_325:0000531
name: banana root nematode density trait
def: "The number of nematode individuals per unit of fresh root weight." [CO:curators]
is_a: TO:0000384 ! nematode damage response trait

[Term]
id: CO_325:0000533
name: banana number of radopholus similis trait
def: "Number of Radopholus similis." [CO:curators]
is_a: TO:0000384 ! nematode damage response trait

[Term]
id: CO_325:0000535
name: banana number of meloidogyne spp. per fresh root weight trait
def: "Number of Meloidogyne spp. in roots." [CO:curators]
is_a: TO:0000384 ! nematode damage response trait

[Term]
id: CO_325:0000537
name: banana number of pratylenchus spp. trait
def: "Number of Pratylenchus spp. in roots." [CO:curators]
is_a: TO:0000384 ! nematode damage response trait

[Term]
id: CO_325:0000539
name: banana number of hoplolaimus spp. per fresh root weight trait
def: "Number of Hoplolaimus spp. in roots." [CO:curators]
is_a: TO:0000384 ! nematode damage response trait

[Term]
id: CO_325:0000541
name: banana number of pratylenchus goodeyi trait
def: "Number of Pratylenchus goodeyi in roots." [CO:curators]
is_a: TO:0000384 ! nematode damage response trait

[Term]
id: CO_325:0000543
name: banana number of pratylenchus coffeae per fresh root weight trait
def: "Number of Pratylenchus coffeae in roots." [CO:curators]
is_a: TO:0000384 ! nematode damage response trait

[Term]
id: CO_325:0000545
name: banana date of first youngest leaf spotted trait
def: "The date a youngest leaf spotted is first observed on the plant, caused by black leaf streak disease." [CO:curators]
is_a: TO:0001145 ! Ascomycete fungal disease response

[Term]
id: CO_325:0000548
name: banana rank of oldest standing leaf trait
def: "The rank (order) of the oldest (most-distal) standing leaf (with an erect petiole)." [CO:curators]
is_a: TO:0000541 ! leaf position

[Term]
id: CO_325:0000550
name: banana date of tagged cigar leaf unrolling at Bruns stage B trait
def: "The date a tagged cigar leaf is at Bruns stage B of unrolling." [CO:curators]
is_a: TO:0000933 ! plant phenological trait

[Term]
id: CO_325:0000553
name: banana date of tagged leaf presenting black leaf streak disease symptoms at Foures stage 1 trait
def: "The date a tagged leaf presents black leaf streak disease symptoms at Foures black leaf streak disease severity grade 1." [CO:curators]
is_a: TO:0001145 ! Ascomycete fungal disease response

[Term]
id: CO_325:0000556
name: banana date of tagged leaf presenting black leaf streak disease symptoms at Foures stage 6 trait
def: "The date a tagged leaf presents black leaf streak disease symptoms at Foures black leaf streak disease severity grade 6." [CO:curators]
is_a: TO:0001145 ! Ascomycete fungal disease response

[Term]
id: CO_325:0000559
name: banana extent of internal discolouration in corm of plant caused by fusarium wilt trait
def: "The extent of discolouration in the corm of the plant, caused by Fusarium wilt." [CO:curators]
is_a: TO:0001145 ! Ascomycete fungal disease response

[Term]
id: CO_325:0000561
name: banana date of first external disease symptoms caused by Fusarium wilt trait
def: "The date of the appearance on the plant of any of the external disease symptoms - yellowing leaves, splitting pseudostem base, changes in new leaves, petiole collapse, caused by Fusarium wilt." [CO:curators]
is_a: TO:0001145 ! Ascomycete fungal disease response

[Term]
id: CO_325:0000564
name: banana rank of marked youngest leaf trait
def: "The rank (position) of the youngest completely unrolled leaf." [CO:curators]
synonym: "rankyoungleaf" EXACT []
is_a: TO:0000541 ! leaf position

[Term]
id: CO_325:0000566
name: banana Rank of previously marked leaf trait
def: "The current rank (position) of the leaf that was previously marked as the youngest leaf at the time of the last data collection event." [CO:curators]
synonym: "rankprevleaf" EXACT []
is_a: TO:0000541 ! leaf position

[Term]
id: CO_325:0000570
name: banana time from planting to first youngest leaf spotted trait
def: "Time elapsed between planting and the appearance of the first youngest leaf spotted." [CO:curators]
is_a: TO:0000933 ! plant phenological trait

[Term]
id: CO_325:0000572
name: banana number of spotted leaves trait
def: "The number of leaves with at least 10 discrete, mature, necrotic lesions or one large necrotic area with 10 light-coloured dry centres, caused by black leaf streak disease." [CO:curators]
synonym: "number and severity of spotted leaves" EXACT []
is_a: TO:0001145 ! Ascomycete fungal disease response

[Term]
id: CO_325:0000574
name: banana black leaf streak disease severity and stage trait
def: "An indication of the extent of damage on an individual leaf caused by black leaf streak disease." [CO:curators]
synonym: "Black Sigatoka disease severity; Percentage area necrotic" EXACT []
synonym: "BLS" EXACT []
is_a: TO:0001145 ! Ascomycete fungal disease response

[Term]
id: CO_325:0000580
name: banana number of leaves with black leaf streak disease severity grade 0 trait
def: "The number of leaves on a plant with a black leaf streak disease severity grade of 0." [CO:curators]
synonym: "number of leaves with black Sigatoka disease severity grade 0" EXACT []
is_a: TO:0001145 ! Ascomycete fungal disease response

[Term]
id: CO_325:0000582
name: banana number of leaves with black leaf streak disease severity grade 1 trait
def: "The number of leaves on a plant with a black leaf streak disease severity grade of 1." [CO:curators]
synonym: "number of leaves with black Sigatoka disease severity grade 1" EXACT []
is_a: TO:0001145 ! Ascomycete fungal disease response

[Term]
id: CO_325:0000584
name: banana number of leaves with black leaf streak disease severity grade 2 trait
def: "The number of leaves on a plant with a black leaf streak disease severity grade of 2." [CO:curators]
synonym: "number of leaves with black Sigatoka disease severity grade 2" EXACT []
is_a: TO:0001145 ! Ascomycete fungal disease response

[Term]
id: CO_325:0000586
name: banana number of leaves with black leaf streak disease severity grade 3 trait
def: "The number of leaves on a plant with a black leaf streak disease severity grade of 3." [CO:curators]
synonym: "number of leaves with black Sigatoka disease severity grade 3" EXACT []
is_a: TO:0001145 ! Ascomycete fungal disease response

[Term]
id: CO_325:0000588
name: banana number of leaves with black leaf streak disease severity grade 4 trait
def: "The number of leaves on a plant with a black leaf streak disease severity grade of 4." [CO:curators]
synonym: "number of leaves with black Sigatoka disease severity grade 4" EXACT []
is_a: TO:0001145 ! Ascomycete fungal disease response


[Term]
id: CO_325:0000590
name: banana number of leaves with black leaf streak disease severity grade 5 trait
def: "The number of leaves on a plant with a black leaf streak disease severity grade of 5." [CO:curators]
synonym: "number of leaves with black Sigatoka disease severity grade 5" EXACT []
is_a: TO:0001145 ! Ascomycete fungal disease response


[Term]
id: CO_325:0000592
name: banana number of leaves with black leaf streak disease severity grade 6 trait
def: "The number of leaves on a plant with a black leaf streak disease severity grade of 6." [CO:curators]
synonym: "number of leaves with black Sigatoka disease severity grade 6" EXACT []
is_a: TO:0001145 ! Ascomycete fungal disease response

[Term]
id: CO_325:0000594
name: banana distance of internal discolouration in pseudostem of tallest sucker caused by fusarium wilt trait
def: "The distance of discolouration in the pseudostem of the tallest sucker, caused by Fusarium wilt." [CO:curators]
is_a: TO:0001145 ! Ascomycete fungal disease response

[Term]
id: CO_325:0000600
name: banana percentage of plants with yellowing leaves caused by fusarium wilt trait
def: "Percentage of plants with yellowing leaves, caused by Fusarium wilt." [CO:curators]
is_a: TO:0001145 ! Ascomycete fungal disease response

[Term]
id: CO_325:0000602
name: banana percentage of plants with a splitting pseudostem base caused by fusarium wilt trait
def: "Percentage of plants with a splitting pseudostem base, caused by Fusarium wilt." [CO:curators]
is_a: TO:0001145 ! Ascomycete fungal disease response

[Term]
id: CO_325:0000604
name: banana percentage of plants with changes in new leaves caused by fusarium wilt trait
def: "Percentage of plants with changes in new leaves, caused by Fusarium wilt." [CO:curators]
is_a: TO:0001145 ! Ascomycete fungal disease response

[Term]
id: CO_325:0000606
name: banana percentage of plants with petiole collapse caused by fusarium wilt trait
def: "Percentage of plants with petiole collapse, caused by Fusarium wilt." [CO:curators]
is_a: TO:0001145 ! Ascomycete fungal disease response

[Term]
id: CO_325:0000650
name: banana Percentage damage to upper cross-section inner corm caused by weevils trait
def: "The amount of damage to the inner corm (central cylinder) upper cross-section, assessed by the percentage of tunnels caused by weevils." [CO:curators]
is_a: TO:0000261 ! insect damage response trait

[Term]
id: CO_325:0000677
name: banana percentage damage to lower cross-section inner corm caused by weevils trait
def: "The amount of damage to the inner corm (central cylinder) lower cross-section, assessed by percentage of tunnels caused by weevils." [CO:curators]
synonym: "Damage index-X-inner" EXACT []
is_a: TO:0000261 ! insect damage response trait

[Term]
id: CO_325:0000679
name: banana percentage damage to lower cross-section outer corm caused by weevils trait
def: "The amount of damage to the outer corm (cortex) lower cross-section, assessed by percentage of tunnels caused by weevils." [CO:curators]
synonym: "Damage index-X-outer" EXACT []
is_a: TO:0000261 ! insect damage response trait

[Term]
id: CO_325:0000726
name: banana weekly leaf emission rate trait
def: "A rate that expresses the number of leaves that have emerged from the pseudostem in a week." [CO:curators]
synonym: "LER" EXACT []
is_a: TTO:0000659 ! phyllochron trait

[Term]
id: CO_325:0000793
name: banana bunch height trait
def: "The height of the bunch." [CO:curators]
synonym: "bunchheight" EXACT []
is_a: TO:1000004 ! infructescence position

[Term]
id: CO_325:0000795
name: banana bunch circumference trait
def: "The circumference of the bunch." [CO:curators]
synonym: "bunchcircumference" EXACT []
is_a: TO:0000920 ! infructescence morphology trait

[Term]
id: CO_325:0000841
name: banana damage to the corm of the mother plant caused by weevils trait
def: "The score of damage to the mother plant corm, assessed by tunnels caused by weevils." [CO:curators]
synonym: "damagemothercorm" EXACT []
is_a: TO:0000261 ! insect damage response trait

[Term]
id: CO_325:0000843
name: banana size of corm inner diameter after weevils introduction trait
def: "The diameter of the inner corm after weevil introduction." [CO:curators]
synonym: "sizeinnercorm" EXACT []
is_a: TO:0000261 ! insect damage response trait

[Term]
id: CO_325:0000845
name: banana size of corm outer diameter after weevils introduction trait
def: "The diameter of the outter corm after weevil introduction." [CO:curators]
synonym: "sizeouttercorm" EXACT []
is_a: TO:0000261 ! insect damage response trait

[Term]
id: CO_325:0000857
name: banana male bud width trait
def: "Width of male bud at its largets point." [CO:curators]
synonym: "Male bud size" EXACT []
is_a: TO:0000789 ! bud morphology trait

[Term]
id: CO_325:0000859
name: banana fruit dry matter content trait
def: "The average dry matter content per unit of fruit fresh weight." [CO:curators]
synonym: "drymattercontent" EXACT []
is_a: TO:0000457 ! biomass yield

[Term]
id: CO_325:0000921
name: banana projected top area trait
def: "The projected leaf area of a plant (photosynthetic surface)." [CO:curators]
synonym: "topLeafArea" EXACT []
is_a: TO:0000540 ! leaf area trait

[Term]
id: CO_325:0000922
name: banana leaf area trait
def: "The area of all leaves." [CO:curators]
synonym: "totLeafArea" EXACT []
is_a: TO:0000540 ! leaf area trait

[Term]
id: CO_325:0000923
name: banana leaf area to plant area ratio trait
def: "Ratio of projected leaf area to the actual leaf area, measure for the compactness of the plant crown." [CO:curators]
synonym: "leafAreaRatio" EXACT []
is_a: TO:0000540 ! leaf area trait

[Term]
id: CO_325:0000924
name: banana total length of all leaves trait
def: "The length of a leaf." [CO:curators]
synonym: "totLeafLength" EXACT []
is_a: TO:0000135 ! leaf length

[Term]
id: CO_325:0000925
name: banana single leaf length trait
def: "The length of a leaf." [CO:curators]
synonym: "singleLeafLength" EXACT []
is_a: TO:0000135 ! leaf length

[Term]
id: CO_325:0000926
name: banana single leaf width trait
def: "The width of a leaf." [CO:curators]
synonym: "singleLeafWidth" EXACT []
is_a: TO:0000370 ! leaf width

[Term]
id: CO_325:0000927
name: banana leaf chlorosis trait
def: "leaf trait correlated to the health stage of the leaf." [CO:curators]
synonym: "leafChlorosis" EXACT []
is_a: TO:0000326 ! leaf color

[Term]
id: CO_325:0000928
name: banana leaf dry weight trait
def: "The dry weight of a leaf." [CO:curators]
synonym: "leafDryMass" EXACT []
is_a: TO:0001014 ! leaf dry weight

[Term]
id: CO_325:0000929
name: banana pseudostem dry weight trait
def: "The dry weight of the pseudostem." [CO:curators]
synonym: "pseudostemDryMass" EXACT []
is_a: TO:0000807 ! pseudostem morphology trait

[Term]
id: CO_325:0000930
name: banana root dry weight trait
def: "The dry weight of the root system." [CO:curators]
synonym: "rootDryMass" EXACT []
is_a: TO:0000078 ! root dry weight

[Term]
id: CO_325:0000931
name: banana plant dry weight trait
def: "The dry weight of the whole plant." [CO:curators]
synonym: "plantDryMass" EXACT []
is_a: TO:0000352 ! plant dry weight

[Term]
id: CO_325:0000932
name: banana ratio root to shoot trait
def: "The ratio of dry mass of belowground (root) to abovegrund (shoot) biomass." [CO:curators]
synonym: "rootShootDry" EXACT []
is_a: TO:0000078 ! root dry weight

[Term]
id: CO_325:0000933
name: banana leaf relative water content trait
def: "The relative water content in a leaf." [CO:curators]
synonym: "rwcLeaf" EXACT []
is_a: TO:0000136 ! leaf relative water content

[Term]
id: CO_325:0000934
name: banana pseudostem relative water content trait
def: "The relative water content in a pseudostem." [CO:curators]
synonym: "rwcPseudostem" EXACT []
is_a: TO:0000807 ! pseudostem morphology trait

[Term]
id: CO_325:0000935
name: banana root relative water content trait
def: "The relative water content in a root." [CO:curators]
synonym: "rwcRoot" EXACT []
is_a: TO:0003036 ! root moisture content

[Term]
id: CO_325:0000936
name: banana plant relative water content trait
def: "The relative water content in the whole plant." [CO:curators]
synonym: "rwcPlant" EXACT []
is_a: TO:0003037 ! plant moisture content

[Term]
id: CO_325:0000937
name: banana pseudostem length trait
def: "The length of a pseudostem." [CO:curators]
synonym: "lengthPseudostem" EXACT []
is_a: TO:0000808 ! pseudostem length

[Term]
id: CO_325:0000938
name: banana leaf number trait
def: "The number of all leaves (including dried/dead/wilted/yellow) in a shoot system." [CO:curators]
synonym: "numLeaves" EXACT []
is_a: TO:0000241 ! leaf number

[Term]
id: CO_325:0000941
name: banana plant water loss trait
def: "The amount of water loss through the plant over time." [CO:curators]
synonym: "waterLossPlant" EXACT []
is_a: TO:0001018 ! transpiration rate

[Term]
id: CO_325:0000942
name: banana transpiration efficiency trait
def: "The growth (weight increase) per volume transpired water." [CO:curators]
synonym: "transpirationEfficiency" EXACT []
is_a: TO:0001017 ! water use efficiency

[Term]
id: CO_325:0000943
name: banana leaf fresh weight trait
def: "A leaf weight trait which is the fresh weight of a leaf." [CO:curators]
synonym: "leafFreshMass" EXACT []
is_a: TO:0000891 ! leaf wet weight

[Term]
id: CO_325:0000944
name: banana pseudostem fresh weight
def: "A pseudostem weight trait which is the fresh weight of a pseudostem." [CO:curators]
synonym: "pseudostemFreshMass" EXACT []
is_a: TO:0000807 ! pseudostem morphology trait

[Term]
id: CO_325:0000945
name: banana root fresh weight trait
def: "A root weight trait which is the fresh weight of a root." [CO:curators]
synonym: "rootFreshMass" EXACT []
is_a: TO:0000578 ! root fresh weight

[Term]
id: CO_325:0000946
name: banana plant fresh weight trait
def: "A plant weight trait which is the fresh weight of a plant." [CO:curators]
synonym: "plantFreshMass" EXACT []
is_a: TO:0000442 ! plant fresh weight

[Term]
id: CO_325:0000947
name: banana leaf to whole plant mass ratio trait
def: "Measure for the biomass allocation: dry mass of leaves versus whole plant dry mass ratio." [CO:curators]
synonym: "leafToPlantMassRatio_dry" EXACT []
is_a: TO:0001014 ! leaf dry weight

[Term]
id: CO_325:0000948
name: banana pseudostem to whole plant mass ratio trait
def: "Measure for the biomass allocation: dry mass of pseudostem versus whole plant dry mass ratio." [CO:curators]
synonym: "pseudostemToPlantMassRatio_dry" EXACT []
is_a: TO:0000807 ! pseudostem morphology trait

[Term]
id: CO_325:0000949
name: banana root to whole plant mass ratio trait
def: "Measure for the biomass allocation: dry mass of roots versus whole plant dry mass ratio." [CO:curators]
synonym: "rootToPlantMassRatio_dry" EXACT []
is_a: TO:0001014 ! leaf dry weight

[Term]
id: CO_325:0000950
name: banana daily rate of water loss trait
def: "The average daily water loss." [CO:curators]
synonym: "waterLossDay" EXACT []
is_a: TO:0001018 ! transpiration rate

[Term]
id: CO_325:0000951
name: banana system water loss per leaf area trait
def: "The amount of water loss in the system normalized by the leaf area." [CO:curators]
synonym: "waterLossSystPerLeafArea" EXACT []
is_a: TO:0001018 ! transpiration rate

[Term]
id: CO_325:0000952
name: banana dry plant growth trait
def: "Dry mass accumulation over time." [CO:curators]
synonym: "growthDry" EXACT []
is_a: TO:0000947 ! whole plant growth and development trait

[Term]
id: CO_325:0000953
name: banana fresh plant growth trait
def: "Fresh mass accumulation over time." [CO:curators]
synonym: "growthFresh" EXACT []
is_a: TO:0000947 ! whole plant growth and development trait

[Term]
id: CO_325:0000954
name: banana increase of leaf area trait
def: "Leaf area increase over time." [CO:curators]
synonym: "leafAreaIncrease" EXACT []
is_a: TO:0000540 ! leaf area trait

[Term]
id: CO_325:0000955
name: banana height increase of pseudostem trait
def: "Pseudostem height increase over time." [CO:curators]
synonym: "pseudostemHeightIncrease" EXACT []
is_a: TO:0000928 ! plant structure growth and development trait

[Term]
id: CO_325:0000956
name: banana pseudostem height increase per leaf formed trait
def: "Stunting expressed as height growth per new formed leaf." [CO:curators]
synonym: "pseudostemHeightIncreasePerFormedLeaf" EXACT []
is_a: TO:0000928 ! plant structure growth and development trait

[Term]
id: CO_325:0000957
name: banana leaves formed per pseudostem height increase trait
def: "Stunting expressed as number of leaves per height growth." [CO:curators]
synonym: "leavesFormedPerPseudostemGrowth" EXACT []
is_a: TO:0000655 ! leaf growth and development trait

[Term]
id: CO_325:0000958
name: banana time from planting to shooting trait
def: "The time elapsed from planting to shooting (when the inflorescence emerges from the pseudostem and is still in an erect position)." [CO:curators]
synonym: "Length of vegetative stage" EXACT []
synonym: "plant2shoot" EXACT []
is_a: TO:0000933 ! plant phenological trait

[Term]
id: CO_325:0000967
name: banana pollen germination trait
def: "The rate of pollen grain germinating." [CO:curators]
synonym: "pollenGerm" EXACT []
is_a: TO:0000421 ! pollen fertility

[Term]
id: CO_325:0000970
name: banana pollen viability trait
def: "The amount of pollen grains which germinate and generate viable plantlets." [CO:curators]
synonym: "pollenVia" EXACT []
is_a: TO:0000421 ! pollen fertility

[Term]
id: CO_325:0000971
name: banana pollen per anther trait
def: "pollen grains per one anther of a male flower." [CO:curators]
synonym: "pollenPerAnth" EXACT []
is_a: TO:1000022 ! anther morphology trait

[Term]
id: CO_325:0000973
name: banana black sigatoka leaf necrosis trait
def: "Black sigatoka leaf symptoms evaluation." [CO:curators]
synonym: "BSLN" EXACT []
is_a: TO:0001145 ! Ascomycete fungal disease response

[Term]
id: CO_325:0000974
name: banana yellow sigatoka leaf necrosis trait
def: "Yellow sigatoka leaf symptoms evaluation." [CO:curators]
synonym: "YSLN" EXACT []
is_a: TO:0001145 ! Ascomycete fungal disease response

[Term]
id: CO_325:0000975
name: banana emusacea leaf spot necrosis trait
def: "Eumusacea leaf spot symptom evaluation." [CO:curators]
synonym: "ELSN" EXACT []
is_a: TO:0001145 ! Ascomycete fungal disease response

[Term]
id: CO_325:0000984
name: banana youngest leaf with streak disease trait
def: "first leaf with first streak disease development stage counted from the first 50% or more of unfurl leaf." [CO:curators]
is_a: TO:0001145 ! Ascomycete fungal disease response

[Term]
id: CO_325:0000985
name: banana pollen grain per anther trait
def: "number of pollen grains per anther." [CO:curators]
is_a: TO:1000022 ! anther morphology trait

[Term]
id: CO_325:0000995
name: banana fruit parthenocarpy trait
is_a: TO:0000929 ! fruit growth and development trait

[Term]
id: CO_325:0000998
name: banana presence of fusarium wilt tropical race 4 trait
def: "The presence of symptoms of fusarium tropical race 4 (foc TR4) on a banana plant." [CO:curators]
is_a: TO:0001145 ! Ascomycete fungal disease response

[Term]
id: CO_325:0001001
name: banana suckering behavior of the plant trait
def: "Banana plant sucker apical dominance type." [CO:curators]
is_a: TO:0000988 ! shoot-borne shoot system morphology trait

[Term]
id: CO_325:0001003
name: banana bunch size trait
def: "The overall size of a banana bunch at mature green stage." [CO:curators]
synonym: "BSZ" EXACT []
is_a: TO:0000920 ! infructescence morphology trait

[Term]
id: CO_325:0001008
name: banana total carotenoids trait
def: "Total caroteinoids with provitamin A activity: pVACs (μg/g)=α-\ncarotene+13-cis-BC+9-cis-BC+trans-BC and TC computed as TC\n(μg/g)=Total pVACs+lutein." [CO:curators]
synonym: "TC" EXACT []
is_a: TO:0000496 ! carotenoid content

[Term]
id: CO_325:0001009
name: banana α-carotene content trait
def: "Content in alpha-carotene quantified by HPLC in ug/g." [CO:curators]
is_a: TO:0002696 ! alpha carotene content

[Term]
id: CO_325:0001010
name: banana 13-cis-beta-carotene content trait
def: "Content in 13-cis-beta-carotene quantified by HPLC in ug/g." [CO:curators]
synonym: "13-cis-BC" EXACT []
is_a: TO:0002695 ! beta-carotene content

[Term]
id: CO_325:0001011
name: banana 9-cis-beta-carotene content trait
def: "Content in 9-cis-beta-carotene quantified by HPLC in ug/g." [CO:curators]
synonym: "9-cis-BC" EXACT []
is_a: TO:0002695 ! beta-carotene content

[Term]
id: CO_325:0001012
name: banana pro-vitamine A content trait
def: "pVACs (μg/g)=α-carotene+13-cis-BC+9-cis-BC+trans-BC." [CO:curators]
synonym: "pVACs" EXACT []
is_a: TO:0000496 ! carotenoid content

[Term]
id: CO_325:0001013
name: banana trans-beta-carotene trait
def: "Content in trans beta- carotene quantified by HPLC in ug/g." [CO:curators]
synonym: "trans-BC" EXACT []
is_a: TO:0002695 ! beta-carotene content

[Term]
id: CO_325:0001014
name: banana lutein content trait
def: "Content in lutein quantified by HPLC in ug/g." [CO:curators]
is_a: TO:0002701 ! lutein content

[Term]
id: CO_325:0002043
name: banana Matooke homogeneity of colour trait
def: "Uniformity of color of the surface of the sample." [CO:curators]
is_a: TO:0000909 ! fruit color uniformity

[Term]
id: CO_325:0002044
name: banana Matooke firmness trait
def: "mechanical textural attribute relating to the force required to achieve a given deformation, penetration, or breakage of a product." [CO:curators]
is_a: TO:0002634 ! fruit firmness

[Term]
id: CO_325:0002045
name: banana Matooke moisture trait
def: "perception of moisture content of a food by the tactile receptors in the mouth and also in relation to the lubricating properties of the product." [CO:curators]
is_a: TO:0003040 ! pepo fruit moisture content

[Term]
id: CO_325:0002046
name: banana Matooke smoothness trait
def: "geometrical textural attribute relating to lack of presence of particles in a product." [CO:curators]
is_a: TO:0001098 ! pepo fruit morphology trait

[Term]
id: CO_325:0002047
name: banana Matooke hardness trait 
def: "mechanical textural attribute relating to the force required to achieve a given deformation, penetration, or breakage of a product." [CO:curators]
is_a: TO:0002634 ! fruit firmness

[Term]
id: CO_325:0002048
name: banana Matooke moldability trait
def: "mechanical textural attribute relating to the degree to which a substance can be deformed before it breaks." [CO:curators]
is_a: TO:0001068 ! processing quality trait

[Term]
id: CO_325:0002049
name: banana Matooke stickiness trait
def: "mechanical textural attribute relating to the force required to remove material that sticks to the mouth." [CO:curators]
is_a: TO:0001068 ! processing quality trait

[Term]
id: CO_325:0002050
name: banana Matooke sweetness trait
def: "basic taste produced by dilute aqueous solutions of natural or artificial substances such as sucrose." [CO:curators]
is_a: TO:0000700 ! fruit sweetness

[Term]
id: CO_325:0002051
name: banana Matooke astringency trait
def: "complex sensation, accompanied by shrinking, drawing or puckering of the skin or mucosal surface in the mouth, produced by substances such as kaki tannins or sloe tannins." [CO:curators]
is_a: TO:0000910 ! fruit bitterness trait

[Term]
id: CO_325:0002052
name: banana Matooke sourness trait
def: "gustatory complex sensation, generally due to presence of organic acids." [CO:curators]
is_a: TO:0002694 ! fruit flavor trait

[Term]
id: CO_325:0002053
name: banana Matooke aroma matooke trait
def: "Aroma of the local matooke." [CO:curators]
is_a: TO:0001068 ! processing quality trait

[Term]
id: CO_325:0002054
name: banana Matooke aroma pumpkin trait
def: "Aroma of pumpkin." [CO:curators]
is_a: TO:0001068 ! processing quality trait

[Term]
id: CO_325:0002055
name: banana Matooke aroma grassy trait
def: "Aroma of fresh grass." [CO:curators]
is_a: TO:0000684 ! grassy flavor

[Term]
id: CO_325:0002056
name: banana Matooke yellowness trait
def: "Color of the surface of the sample from light yellow to bright yellow." [CO:curators]
is_a: TO:0002617 ! fruit color

[Term]
id: CO_325:0003000
name: banana raw pulp color trait
def: "A quick field evaluation of the raw pulp to determine acceptability based on yellow color using Mbwazirume as a standard control." [CO:curators]
is_a: TO:0002617 ! fruit color

[Term]
id: CO_325:0003003
name: banana sap amount trait
def: "A quick field evaluation of the raw pulp to determine acceptability based on yellow color using Mbwazirume as a standard control." [CO:curators]
is_a: TO:0001098 ! pepo fruit morphology trait

[Term]
id: CO_325:0003004
name: banana weevil damage assessment trait
def: "Weevil damage assesssment." [CO:curators]
is_a: TO:0000261 ! insect damage response trait

[Term]
id: CO_325:0003014
name: banana nematode damage trait
is_a: TO:0000384 ! nematode damage resistance

[Term]
id: CO_325:0003015
name: banana Helicotylincus mulicinctus damage trait
def: "Helicotylincus mulicinctus damage assesssment." [CO:curators]
is_a: TO:0000384 ! nematode damage resistance

[Term]
id: CO_325:0003019
name: banana Radopholus similis damage trait
def: "Radopholus similis damage assesssment." [CO:curators]
is_a: TO:0000384 ! nematode damage resistance

[Term]
id: CO_325:0003023
name: banana Pratylenchus goodeyi damage trait
def: "Pratylenchus goodeyi damage assesssment." [CO:curators]
is_a: TO:0000384 ! nematode damage resistance

[Term]
id: CO_325:0003028
name: banana fruit acceptability trait
def: "A general take of the panelist about the sample after the aroma, colour, taste, and mouth-feel specific tests." [CO:curators]
is_a: TO:0000322 ! phenotypic acceptability

[Term]
id: CO_325:0003030
name: banana weevil insect assessment trait
def: "Weevil insect assesssment." [CO:curators]
is_a: TO:0000261 ! insect damage response trait

[Term]
id: CO_325:0003034
name: banana number of helicotylenchus multicinctus trait
def: "number of Helicotylenchus multicinctus in root." [CO:curators]
is_a: TO:0000384 ! nematode damage resistance

[Term]
id: CO_325:0003037
name: banana Pratylenchus spp. damage trait
def: "Pratylenchus spp. damage assesssment." [CO:curators]
is_a: TO:0000384 ! nematode damage resistance

[Term]
id: CO_325:0003038
name: banana Pratylenchus coffeae damage trait
def: "Pratylenchus coffeae damage assesssment." [CO:curators]
is_a: TO:0000384 ! nematode damage resistance

[Term]
id: CO_325:0003045
name: banana insect damage trait
is_a: TO:0000261 ! insect damage response trait

[Term]
id: CO_325:0003046
name: banana bacterial damage trait
is_a: TO:0000315 ! bacterial disease response

[Term]
id: CO_325:0003047
name: banana xanthomonas wilt damage trait
def: "banana xanthomonas wilt damage assesssment." [CO:curators]
synonym: "BXW" EXACT []
is_a: TO:0000315 ! bacterial disease response

[Term]
id: CO_325:0003055
name: banana damage to upper cross-section inner corm caused by weevils trait
def: "Damage to the inner corm (central cylinder) upper cross-section caused by weevils." [CO:curators]
is_a: TO:0000261 ! insect damage response trait

[Term]
id: CO_325:0003056
name: banana damage to upper cross-section outer corm caused by weevils trait
def: "Damage to the outer corm (cortex) upper cross-section caused by weevils." [CO:curators]
is_a: TO:0000261 ! insect damage response trait

[Term]
id: CO_325:0003057
name: banana fertility trait
def: "n/a." [CO:curators]
is_a: TO:0000392 ! sterility or fertility trait

[Term]
id: CO_325:0003058
name: banana female fertility trait
def: "n/a." [CO:curators]
is_a: TO:0000392 ! sterility or fertility trait

[Term]
id: CO_325:0003059
name: banana male fertility trait
def: "n/a." [CO:curators]
is_a: TO:0000392 ! sterility or fertility trait

[Term]
id: CO_325:0003064
name: banana number of dead leaves trait
def: "The number of dead leaves on the plant." [CO:curators]
is_a: TO:0000250 ! plant vigor trait

[Term]
id: CO_325:0003066
name: banana rhizome weight trait
def: "corm weight." [CO:curators]
synonym: "corm weight" EXACT []
is_a: TO:0000568 ! shoot axis weight

[Term]
id: CO_325:0003074
name: banana damage to the pseudostem caused by weevils trait
def: "Does weevil damage extend into the pseudostem." [CO:curators]
is_a: TO:0000261 ! insect damage response trait

[Term]
id: CO_325:0003082
name: banana plant stature trait
def: "A ratio of plant circumference to plant height." [CO:curators]
is_a: TO:1000012 ! whole plant size

[Term]
id: CO_325:0003106
name: banana boiled plantain textural characteristic hardness trait
def: "The amount of force required to deform or to overcome resistance to puncture of the food material. Hardness is determined as the highest peak force in g measured during the first TPA compression." [CO:curators]
xref: https://doi.org/10.18167/agritrop/00685
is_a: TO:0001069 ! cooking quality trait

[Term]
id: CO_325:0003108
name: banana boiled plantain textural characteristic distance at Fmax trait
def: "The depth at which the hardness of boiled plantain is registered. It represents the the distance into the sample where hardness is the highest. High distances mean the sample has softer pulp. A proxy for firmness which is the property of a food material being unyielding to touch." [CO:curators]
xref: https://doi.org/10.18167/agritrop/00685
is_a: TO:0001069 ! cooking quality trait

[Term]
id: CO_325:0003109
name: banana boiled plantain textural characteristic penetration area trait
def: "Work done or energy required to penetrate the boiled plantain sample. It represents the amount of energy that must be expended to penetrate the sample. Work done to penetrate sample in g.mm determined as total area under the curve." [CO:curators]
xref: https://doi.org/10.18167/agritrop/00685
is_a: TO:0001069 ! cooking quality trait

[Term]
id: CO_325:0003110
name: banana boiled plantain textural characteristic distance to max force first TPA compression trait
def: "Textural parameter used to calculate springness. It represents the depth of the sample where hardness is registered on first compression cycle. Textural parameter used to calculate cheweness and springness." [CO:curators]
xref: https://doi.org/10.18167/agritrop/00685
is_a: TO:0001069 ! cooking quality trait

[Term]
id: CO_325:0003111
name: banana boiled plantain textural characteristic distance to max force second TPA compression trait
def: "Textural parameter used to calculate springness. It represents the depth of the sample where hardness is registered on second compression cycle. The distance in mm between the beginning of the second compression and the highest peak force of the second compression." [CO:curators]
xref: https://doi.org/10.18167/agritrop/00685
is_a: TO:0001069 ! cooking quality trait

[Term]
id: CO_325:0003112
name: banana boiled plantain textural characteristic area under curve first compression trait
def: "Textural parameter used to calculate cohesiveness and resilience. It represents the work done to compress sample on first compression cycle. The area underneath the curve in g.mm between beginning of first compression and highest peak force of first compression." [CO:curators]
xref: https://doi.org/10.18167/agritrop/00685
is_a: TO:0001069 ! cooking quality trait

[Term]
id: CO_325:0003113
name: banana boiled plantain textural characteristic area under curve first withdrawal trait
def: "Textural parameter used to calculate cohesiveness and resilience. It represents the work done to decompress sample on first withdrawal cycle. The area underneath the curve in g.mm between highest peak force of first compression and end of first withdrawal." [CO:curators]
xref: https://doi.org/10.18167/agritrop/00685
is_a: TO:0001069 ! cooking quality trait

[Term]
id: CO_325:0003114
name: banana boiled plantain textural characteristic area under curve second compression trait
def: "Textural parameter used to calculate cohesiveness. It represents the work done to compress sample on second compression cycle. The area underneath the curve in g.mm between beginning of second compression and highest peak force of second compression." [CO:curators]
xref: https://doi.org/10.18167/agritrop/00685
is_a: TO:0001069 ! cooking quality trait

[Term]
id: CO_325:0003115
name: banana boiled plantain textural characteristic area under curve second withdrawal trait
def: "Textural parameter used to calculate cohesiveness. It represents the work done to decompress sample on second withdrawal cycle. The area underneath the curve in g.mm between highest peak force of second compression and end of second withdrawal." [CO:curators]
xref: https://doi.org/10.18167/agritrop/00685
is_a: TO:0001069 ! cooking quality trait

[Term]
id: CO_325:0003116
name: banana boiled plantain textural characteristic adhesiveness/stickness trait
def: "The work required in overcoming the attractive force between a product and the contact surface.  It represents how sticky the boiled plantain sample is. Adhesiveness is represented by the area in g.s covered by the first negative peak (c)." [CO:curators]
xref: https://doi.org/10.18167/agritrop/00685
is_a: TO:0001069 ! cooking quality trait

[Term]
id: CO_325:0003117
name: banana boiled plantain textural characteristic cohesiveness trait
def: "The work required to overcome the internal bonds of a material. It represents the ability of the boiled plantain sample to remain compact and not fracture or disintegrate into bits. Cohesiveness is calculated as area underneath the second compression and withdrawal curves divided by the area underneath the first compression and withdrawal curves [(d+e)/(a+b)]." [CO:curators]
xref: https://doi.org/10.18167/agritrop/00685
is_a: TO:0001069 ! cooking quality trait

[Term]
id: CO_325:0003118
name: banana boiled plantain textural characteristic springiness trait
def: "The degree to which food can recover between the end of the first bite and the beginning of the second bite in the mouth. Springiness represents the ability of boiled plantain to regain its ''elastic'' nature after compression. Springness is calculated as a ratio or percentage of a product’s recovery to its original height [(Distance 2)/(Distance 1)]*100 or (Time 2/Time 1)*100." [CO:curators]
xref: https://doi.org/10.18167/agritrop/00685
is_a: TO:0001069 ! cooking quality trait

[Term]
id: CO_325:0003119
name: banana boiled plantain textural characteristic gumminess trait
def: "Mechanical textural attribute related to the cohesiveness of a tender product. The product of cohesiveness and hardness calculated from Hardness x Cohesiveness F1*[(d+e)/(a+b)]." [CO:curators]
xref: https://doi.org/10.18167/agritrop/00685
is_a: TO:0001069 ! cooking quality trait

[Term]
id: CO_325:0003120
name: banana boiled plantain textural characteristic chewiness trait
def: "The mechanical textural attribute related to the amount of work required to masticate a solid. It is the product of gumminess and springiness. Cheweness is calculated from Hardness x Cohesiveness x Springiness (F1*((d+e)/(a+b))*(Distance 2/Distance 1))." [CO:curators]
xref: https://doi.org/10.18167/agritrop/00685
is_a: TO:0001069 ! cooking quality trait

[Term]
id: CO_325:0003121
name: banana boiled plantain textural characteristic resilience trait
def: "The mechanical textural attribute relating to the rapidity of recovery from a deforming force or the degree to which a deformed material returns to its original condition after the deforming force is removed. The textural attribute representing the ability of boiled plantain to recover to its original size after compression." [CO:curators]
xref: https://doi.org/10.18167/agritrop/00685
is_a: TO:0001069 ! cooking quality trait

[Term]
id: CO_325:0120047
name: banana boiled plantain firmness trait
def: "Force required to obtain deformation, penetration or rupture of the banana." [CO:curators]
is_a: TO:0001069 ! cooking quality trait

[Term]
id: CO_325:0120051
name: banana boiled plantain chewiness trait
def: "Energy or number of chews necessary to chew the banana to make it ready to be swallowed." [CO:curators]
is_a: TO:0001069 ! cooking quality trait

[Term]
id: CO_325:0120055
name: banana boiled plantain mealiness trait
def: "Mechanical property linked to cohesion and the presence of fine particles in the product during chewing." [CO:curators]
is_a: TO:0001069 ! cooking quality trait

[Term]
id: CO_325:0120059
name: banana boiled plantain stickiness trait
def: "Force required to peel off the fraction of product adhering to the interior of the oral cavity." [CO:curators]
is_a: TO:0001069 ! cooking quality trait

[Term]
id: CO_325:0120063
name: banana boiled plantain sweetness trait
def: "Elemental flavor caused by dilute aqueous solutions of various substances such as sucrose or aspartame." [CO:curators]
is_a: TO:0001069 ! cooking quality trait

[Term]
id: CO_325:0120067
name: banana boiled plantain moistness trait
def: "Perception of the amount of water absorbed or released by the product. [CO:curators]"
is_a: TO:0001069 ! cooking quality trait
